Snapshot. Not working and becoming too complicated.

src/dafny/refinement/evm.dfy
@@ -63,7 +63,8 @@ module EVM {
      *  @param  p   The program to be executed.
      *  @param  s   The initial state.
      *  @param  n   The maximum number of steps to be executed.
-     *  @returns    The state reached from `s` by executing at most `n` steps of `p`.
+     *  @returns    The state reached from `s` by executing at most `n` steps of `p` and 
+     *              the last pc.
      *
      *  @note       In this semantics `jumps` are relative i.e. `jump(k)` updates the 
      *              `pc` to `pc + k`.
@@ -81,6 +82,40 @@ module EVM {
                 case Jumpi(c, tgt)  =>  if !c(s) then runEVM2(pc + 1, p, s, n - 1) 
                                         else runEVM2(pc + tgt, p, s, n - 1)
                 case Jump(tgt)      =>  runEVM2(pc + tgt, p, s, n - 1) 
+    }
+
+    //  returns s', pc', n'
+    function method runEVM3<S>(pc: int, p: seq<EVMProg2>, s: S, n: nat): (S, int, nat)
+        decreases n 
+    {
+        if n == 0 || pc >= |p| || pc < 0 then (s, pc, n)
+            //  We could have different types of termination.
+        else 
+            //  Execute instruction at PC and increment PC accordingly.
+            match p[pc] 
+                case AInst(i)       =>  runEVM3(pc + 1, p, runInst(i, s), n - 1)
+                case Jumpi(c, tgt)  =>  if !c(s) then runEVM3(pc + 1, p, s, n - 1) 
+                                        else runEVM3(pc + tgt, p, s, n - 1)
+                case Jump(tgt)      =>  runEVM3(pc + tgt, p, s, n - 1) 
+    }
+
+    /**
+     *  Run one step of a program.
+     *  
+     *
+     *  @note   If the `pc` is outside the sdt of instructions, stop.
+     */
+    function method stepEVM<S>(pc: nat, p: seq<EVMProg2>, s: S): (int, S)
+    {
+        if pc < 0 || pc >= |p| then  
+            (pc, s)
+        else 
+            match p[pc] 
+                case AInst(i)       =>  (pc + 1, runInst(i, s))
+                case Jumpi(c, tgt)  =>  if !c(s) then (pc + 1, s) 
+                                        else (pc + tgt, s)
+                case Jump(tgt)      =>  (pc + tgt, s) 
+
     }
 
     /**
@@ -116,14 +151,19 @@ module EVM {
 
     /**
      *  The execution of n steps of a closed program |p| either termninates with 
-     *  pc in 0..|p| - 1 and n == 0 or pc == |p| and n >= 0 
+     *  pc in 0..|p| - 1 and n == 0 or pc == |p| and n >= 0.
+     *
+     *  @param  pc  An initial pc.
+     *  @param  p   An EVM program.
+     *  @param  s   An initial state.
+     *  @param  n   The maximum number of steps to be executed.
      */
-    lemma pcBoundsOnTernination<S>(pc: nat, p: seq<EVMProg2>, s: S, n:nat) 
+    lemma pcBoundsOnTermination<S>(pc: nat, p: seq<EVMProg2>, s: S, n: nat) 
         requires isClosed(p)
         requires 0 <= pc <= |p|
-        ensures 0 <= runEVM2<S>(pc, p, s, n).1 <= |p|
-        ensures 0 <= runEVM2<S>(pc, p, s, n).1 < |p| ==> n == 0
-        ensures runEVM2<S>(pc, p, s, n).1 == |p| ==> n >= 0  
+        ensures 0 <= runEVM3<S>(pc, p, s, n).1 <= |p|
+        ensures 0 <= runEVM3<S>(pc, p, s, n).1 < |p| ==> runEVM3<S>(pc, p, s, n).2 == 0 
+        ensures runEVM3<S>(pc, p, s, n).1 == |p| ==> runEVM3<S>(pc, p, s, n).2 >= 0  
         decreases n 
     {
         if |p| == pc || n == 0 {
@@ -132,15 +172,76 @@ module EVM {
             assert pc < |p|; 
             match p[pc] 
                 case AInst(i)           =>  
-                    pcBoundsOnTernination(pc + 1, p, runInst(i, s), n - 1);
+                    pcBoundsOnTermination(pc + 1, p, runInst(i, s), n - 1);
                 case Jumpi(cond, tgt)   =>  
                     assert closeJump(p, pc);
                     assert 0 <= pc + tgt <= |p|;
-                    pcBoundsOnTernination(if cond(s) then pc + tgt else pc + 1, p, s, n - 1);
+                    pcBoundsOnTermination(if cond(s) then pc + tgt else pc + 1, p, s, n - 1);
                 case Jump(tgt)          => 
                     assert closeJump(p, pc);
                     assert 0 <= pc + tgt <= |p|;
-                    pcBoundsOnTernination(pc + tgt, p, s, n - 1);
+                    pcBoundsOnTermination(pc + tgt, p, s, n - 1);
         }
     }
+
+    lemma localProp<S>(pc: nat, p: seq<EVMProg2>, s: S, k1: nat, k2: nat)
+        requires 0 <= k1 < k2 < |p|
+        requires isClosed(p[k1..k2])
+        requires k1 <= pc < k2
+        ensures k1 <= stepEVM(pc, p, s).0 <= k2 
+        // decreases n
+    {
+        if false {
+            //  Thanks Dafny
+        } else if pc == k2 { 
+            // calc <= {
+            //     runEVM3(pc, p, s, n).1;
+            //     runEVM3(pc, p[k1..k2], s, n).1;
+            //     // { assert isClosed(p[k1..k2]) ;}
+            //     // k2;
+            // }
+        } else {
+            assert k1 <= pc < k2; 
+            match p[pc] 
+                case AInst(i)           =>  
+                    // localProp(pc + 1, p, runInst(i, s), k1, k2);
+                    // assume k1 <= runEVM3(k1, p, s, n).1 <= k2 ;
+                    // pcBoundsOnTermination(pc + 1, p, runInst(i, s), n - 1);
+                case Jumpi(cond, tgt)   =>  
+                    // assert closeJump(p, pc);
+                    assume k1 <= stepEVM(pc, p, s).0 <= k2 ;
+                    // assert 0 <= pc + tgt <= |p|;
+                    // pcBoundsOnTermination(if cond(s) then pc + tgt else pc + 1, p, s, n - 1);
+                case Jump(tgt)          => 
+                    // assume k1 <= stepEVM(pc, p, s).0 <= k2 ;
+                    calc == {
+                        p[pc];
+                        p[k1..k2][pc - k1];
+                    }
+                    calc == {
+                        stepEVM(pc, p, s);
+                        (pc + tgt, s);
+                        calc == {
+                            p[pc];
+                            p[k1..k2][pc - k1];
+                        }
+                        stepEVM(pc - k1, p[k1..k2], s);
+                        // (pc + tgt, s);
+                    }
+                    calc == {
+                        stepEVM(pc - k1, p[k1..k2], s).0;
+                        pc - k1 + tgt;
+                        // calc == {
+                        //     p[pc];
+                        //     p[k1..k2][pc - k1];
+                        // }
+
+                    }
+                    assume k1 <= stepEVM(pc, p, s).0 <= k2 ;
+                    // assert closeJump(p[k1..k2], pc);
+                    // assert 0 <= pc + tgt <= |p|;
+                    // pcBoundsOnTermination(pc + tgt, p, s, n - 1);
+                    // assume k1 <= runEVM3(k1, p, s, n).1 <= k2 ;
+        }   
+    } 
 }
